Almost there with type preservation, tho still missing the actual type (substitution lemma)

theories/abs_defs.v
@@ -131,6 +131,15 @@ Fixpoint fresh_vars_s (l : list x) (s0 : s): Prop :=
 Definition fresh_vars (l : list x) (e0: e) (s0: s) : Prop :=
   fresh_vars_s l s0 /\ fresh_vars_e l e0.
 
+Inductive distinct: list x -> Prop :=
+ | distinct_nil: distinct nil
+ | distinct_cons: forall y ys,
+      ~ In y ys ->
+     distinct ys ->
+     distinct (y::ys).
+
+Definition well_formed (e0: e) (s0: s) (l:list x) : Prop := fresh_vars l e0 s0 /\ distinct l.
+
 (** definitions *)
 
 (* defns expression_well_typing *)
@@ -165,7 +174,7 @@ Inductive red_e : list F -> s -> e -> s -> e -> Prop :=    (* defn e *)
      red_e F_list s5 e_5 s' e' ->
      red_e F_list s5 (e_fn_call fn5 ((app e_list (app (cons e_5 nil) (app e'_list nil))))) s' (e_fn_call fn5 ((app e_list (app (cons e' nil) (app e'_list nil)))))
  | red_fun_ground : forall (T_x_t_y_list:list (T*x*t*x)) (F'_list F_list:list F) (T_5:T) (fn5:fn) (e5:e) (s5:s),
-      (fresh_vars  (map (fun (pat_:(T*x*t*x)) => match pat_ with (T_,x_,t_,y_) => y_ end ) T_x_t_y_list)   e5   s5 )  ->
+      (well_formed  e5   s5   (map (fun (pat_:(T*x*t*x)) => match pat_ with (T_,x_,t_,y_) => y_ end ) T_x_t_y_list) )  ->
      red_e ((app F_list (app (cons (F_fn T_5 fn5 (map (fun (pat_:(T*x*t*x)) => match pat_ with (T_,x_,t_,y_) => (T_,x_) end ) T_x_t_y_list) e5) nil) (app F'_list nil)))) s5 (e_fn_call fn5 (map (fun (pat_:(T*x*t*x)) => match pat_ with (T_,x_,t_,y_) => (e_t t_) end ) T_x_t_y_list))  (fold_right (fun (xt : x * t) (s5 : s) => Map.add (fst xt) (snd xt) s5)  s5   (map (fun (pat_:(T*x*t*x)) => match pat_ with (T_,x_,t_,y_) => (y_,t_) end ) T_x_t_y_list) )   (e_var_subst  e5   (map (fun (pat_:(T*x*t*x)) => match pat_ with (T_,x_,t_,y_) => (x_,y_) end ) T_x_t_y_list) ) .
 
 
